symbolic_state_cmp_impl.v
@@ -1,0 +1,79 @@
+Require Import Arith.
+Require Import Nat.
+Require Import Bool.
+Require Import bbv.Word.
+Require Import Coq.NArith.NArith.
+Require Import List.
+Import ListNotations.
+
+Require Import FORVES2.constants.
+Import Constants.
+
+Require Import FORVES2.program.
+Import Program.
+
+Require Import FORVES2.execution_state.
+Import ExecutionState.
+
+Require Import FORVES2.stack_operation_instructions.
+Import StackOpInstrs.
+
+Require Import FORVES2.misc.
+Import Misc.
+
+Require Import FORVES2.symbolic_state.
+Import SymbolicState.
+
+Require Import FORVES2.symbolic_state_eval.
+Import SymbolicStateEval.
+
+
+Require Import FORVES2.valid_symbolic_state.
+Import ValidSymbolicState.
+
+Require Import FORVES2.valid_symbolic_state.
+Import ValidSymbolicState.
+
+Require Import FORVES2.symbolic_state_cmp.
+Import SymbolicStateCmp.
+
+Require Import FORVES2.eval_common.
+Import EvalCommon.
+
+Require Import FORVES2.constraints.
+Import Constraints.
+
+Module SymbolicStateCmpImpl.
+
+Definition compare_sstack (sstack_val_cmp: sstack_val_cmp_t) (ctx: constraints)  (sstk1 sstk2: sstack) (maxidx1: nat) (sb1: sbindings) (maxidx2: nat) (sb2: sbindings) (ops: stack_op_instr_map) : bool :=
+  fold_right_two_lists (fun e1 e2 => sstack_val_cmp ctx e1 e2 maxidx1 sb1 maxidx2 sb2 ops) sstk1 sstk2.
+
+Definition compare_smemory (smemory_cmp: smemory_cmp_t) (ctx: constraints)  (smem1 smem2: smemory) (maxidx1: nat) (sb1: sbindings) (maxidx2: nat) (sb2: sbindings) (ops: stack_op_instr_map) : bool :=
+  smemory_cmp ctx smem1 smem2 maxidx1 sb1 maxidx2 sb2 ops.
+
+Definition compare_sstorage (sstorage_cmp: sstorage_cmp_t) (ctx: constraints) (sstrg1 sstrg2: sstorage) (maxidx1: nat) (sb1: sbindings) (maxidx2: nat) (sb2: sbindings) (ops: stack_op_instr_map) : bool :=
+      sstorage_cmp ctx sstrg1 sstrg2 maxidx1 sb1 maxidx2 sb2 ops.
+
+
+Definition sstate_cmp (sstack_val_cmp: sstack_val_cmp_t) (smemory_cmp: smemory_cmp_t) (sstorage_cmp: sstorage_cmp_t) (ctx: constraints) (sst1 sst2: sstate) (ops: stack_op_instr_map) : bool :=
+  let sstk1 := get_stack_sst sst1 in
+  let smem1 := get_memory_sst sst1 in 
+  let sstrg1 := get_storage_sst sst1 in
+  let m1 := get_smap_sst sst1 in
+  let maxidx1 := get_maxidx_smap m1 in
+  let sb1 := get_bindings_smap m1 in
+  let sstk2 := get_stack_sst sst2 in
+  let smem2 := get_memory_sst sst2 in 
+  let sstrg2 := get_storage_sst sst2 in
+  let m2 := get_smap_sst sst2 in
+  let maxidx2 := get_maxidx_smap m2 in
+  let sb2 := get_bindings_smap m2 in
+  if compare_sstack sstack_val_cmp ctx sstk1 sstk2 maxidx1 sb1 maxidx2 sb2 ops then
+    if compare_smemory smemory_cmp ctx smem1 smem2 maxidx1 sb1 maxidx2 sb2 ops then
+      if compare_sstorage sstorage_cmp ctx sstrg1 sstrg2 maxidx1 sb1 maxidx2 sb2 ops then
+        true
+      else false
+    else false
+  else false.
+         
+End SymbolicStateCmpImpl.
