symbolic_state_cmp_impl_soundness.v
@@ -1,0 +1,170 @@
+Require Import Arith.
+Require Import Nat.
+Require Import Bool.
+Require Import bbv.Word.
+Require Import Coq.NArith.NArith.
+Require Import List.
+Import ListNotations.
+
+Require Import FORVES2.constants.
+Import Constants.
+
+Require Import FORVES2.program.
+Import Program.
+
+Require Import FORVES2.execution_state.
+Import ExecutionState.
+
+Require Import FORVES2.stack_operation_instructions.
+Import StackOpInstrs.
+
+Require Import FORVES2.misc.
+Import Misc.
+
+Require Import FORVES2.symbolic_state.
+Import SymbolicState.
+
+Require Import FORVES2.symbolic_state_eval.
+Import SymbolicStateEval.
+
+
+Require Import FORVES2.valid_symbolic_state.
+Import ValidSymbolicState.
+
+Require Import FORVES2.valid_symbolic_state.
+Import ValidSymbolicState.
+
+Require Import FORVES2.symbolic_state_cmp.
+Import SymbolicStateCmp.
+
+Require Import FORVES2.symbolic_state_cmp_impl.
+Import SymbolicStateCmpImpl.
+
+Require Import FORVES2.eval_common.
+Import EvalCommon.
+
+Require Import FORVES2.constraints.
+Import Constraints.
+
+Module SymbolicStateCmpSoundness.
+
+  Lemma sstack_cmp_snd:
+    forall sstack_val_cmp ctx sstk1 sstk2 maxidx1 sb1 maxidx2 sb2 ops,
+      is_sat ctx ->
+      valid_sstack maxidx1 sstk1 ->
+      valid_sstack maxidx2 sstk2 ->
+      valid_bindings maxidx1 sb1 ops ->
+      valid_bindings maxidx2 sb2 ops ->
+      safe_sstack_val_cmp sstack_val_cmp ->
+      fold_right_two_lists (fun e1 e2 : sstack_val => sstack_val_cmp ctx e1 e2 maxidx1 sb1 maxidx2 sb2 ops) sstk1 sstk2 = true ->
+      forall model mem strg exts,
+        is_model ctx model = true ->
+        exists v,
+          eval_sstack sstk1 maxidx1 sb1 model mem strg exts ops = Some v /\
+            eval_sstack sstk2 maxidx2 sb2 model mem strg exts ops = Some v.
+
+  Proof.
+    intro sstack_val_cmp.
+    induction sstk1 as [|sv1 sstk1' IHsstk1'].
+    - intros.
+      destruct sstk2.
+      + simpl. exists []. split; reflexivity.
+      + discriminate.
+    - intros sstk2 maxidx1 sb1 maxidx2 sb2 ops H_is_sat H_valid_sstk1 H_valid_sstk2 H_valid_sb1 H_valid_sb2 H_safe_sstack_val_cmp H_fold.
+
+      intros model mem strg exts H_is_model.
+
+      destruct sstk2 as [|sv2 sstk2']; try discriminate.
+      simpl in H_fold.
+      destruct (sstack_val_cmp ctx sv1 sv2 maxidx1 sb1 maxidx2 sb2 ops) eqn:E_cmp_sv1_sv2; try discriminate.
+
+
+      assert (H_safe_sstack_val_cmp' := H_safe_sstack_val_cmp).
+      unfold safe_sstack_val_cmp in H_safe_sstack_val_cmp'.
+      simpl in H_valid_sstk1.
+      destruct H_valid_sstk1 as [H_valid_sv1 H_valid_sstk1'].
+      
+      simpl in H_valid_sstk2.
+      destruct H_valid_sstk2 as [H_valid_sv2 H_valid_sstk2'].
+
+      pose proof (H_safe_sstack_val_cmp' ctx sv1 sv2 maxidx1 sb1 maxidx2 sb2 ops H_is_sat H_valid_sv1 H_valid_sv2 H_valid_sb1 H_valid_sb2 E_cmp_sv1_sv2 model mem strg exts H_is_model) as H_safe_sstack_val_cmp'.
+      destruct H_safe_sstack_val_cmp' as [v [H_eval_sv1 H_eval_sv2]].
+      pose proof (IHsstk1' sstk2' maxidx1 sb1 maxidx2 sb2 ops H_is_sat H_valid_sstk1' H_valid_sstk2' H_valid_sb1 H_valid_sb2 H_safe_sstack_val_cmp H_fold model mem strg exts H_is_model) as IHsstk1'_0.
+      destruct IHsstk1'_0 as [l [H_eval_sstk1' H_eval_sstk2']].
+      simpl eval_sstack.
+      rewrite H_eval_sv1.
+      rewrite H_eval_sv2.
+      rewrite H_eval_sstk1'.
+      rewrite H_eval_sstk2'.
+      exists  (v :: l).
+      split; reflexivity.
+  Qed.
+
+      
+    
+                                                                     
+  Lemma sstate_cmp_snd:
+    forall sstack_val_cmp smemory_cmp sstorage_cmp,
+      safe_sstack_val_cmp sstack_val_cmp ->
+      safe_smemory_cmp smemory_cmp ->
+      safe_sstorage_cmp sstorage_cmp ->
+      symbolic_state_cmp_snd (sstate_cmp sstack_val_cmp smemory_cmp sstorage_cmp).
+  Proof.
+    intros sstack_val_cmp smemory_cmp sstorage_cmp H_safe_sstack_val_cmp H_safe_smemory_cmp H_safe_sstorage_cmp.
+    unfold symbolic_state_cmp_snd.
+    intros ctx sst1 sst2 ops H_is_sat H_valid_sst1 H_valid_sst2 H_sstate_cmp mem strg exts model H_is_model.
+
+    unfold sstate_cmp in H_sstate_cmp.
+    
+    destruct (compare_sstack sstack_val_cmp ctx (get_stack_sst sst1) (get_stack_sst sst2) (get_maxidx_smap (get_smap_sst sst1)) (get_bindings_smap (get_smap_sst sst1)) (get_maxidx_smap (get_smap_sst sst2)) (get_bindings_smap (get_smap_sst sst2)) ops) eqn:E_sstack_cmp; try discriminate.
+
+    destruct (compare_smemory smemory_cmp ctx (get_memory_sst sst1) (get_memory_sst sst2) (get_maxidx_smap (get_smap_sst sst1)) (get_bindings_smap (get_smap_sst sst1)) (get_maxidx_smap (get_smap_sst sst2)) (get_bindings_smap (get_smap_sst sst2)) ops) eqn:E_smemory_cmp; try discriminate.
+
+    destruct (compare_sstorage sstorage_cmp ctx (get_storage_sst sst1) (get_storage_sst sst2) (get_maxidx_smap (get_smap_sst sst1)) (get_bindings_smap (get_smap_sst sst1)) (get_maxidx_smap (get_smap_sst sst2)) (get_bindings_smap (get_smap_sst sst2)) ops) eqn:E_sstorage_cmp; try discriminate.
+
+    unfold valid_sstate in H_valid_sst1.
+    unfold valid_smap in H_valid_sst1.
+    destruct H_valid_sst1 as [H_valid_sst1_sb [H_valid_sstack_sst1 [H_valid_smemory_sst1 H_valid_sstorage_sst1]]].
+
+    unfold valid_sstate in H_valid_sst2.
+    unfold valid_smap in H_valid_sst2.
+    destruct H_valid_sst2 as [H_valid_sst2_sb [H_valid_sstack_sst2 [H_valid_smemory_sst2 H_valid_sstorage_sst2]]].
+
+    unfold eval_sstate.
+
+    (* storage *)
+    unfold compare_sstorage in E_sstorage_cmp.
+    unfold safe_sstorage_cmp in H_safe_sstorage_cmp.
+    pose proof (H_safe_sstorage_cmp ctx (get_storage_sst sst1) (get_storage_sst sst2) (get_maxidx_smap (get_smap_sst sst1)) (get_bindings_smap (get_smap_sst sst1)) (get_maxidx_smap (get_smap_sst sst2)) (get_bindings_smap (get_smap_sst sst2)) ops H_is_sat H_valid_sst1_sb H_valid_sst2_sb H_valid_sstorage_sst1 H_valid_sstorage_sst2 E_sstorage_cmp) as H_safe_sstorage_cmp.
+
+    pose proof (H_safe_sstorage_cmp model mem strg exts H_is_model) as H_safe_sstorage_cmp.
+    destruct H_safe_sstorage_cmp as [strg' [H_safe_sstorage_cmp_0 H_safe_sstorage_cmp_1]].
+    rewrite H_safe_sstorage_cmp_0.
+    rewrite H_safe_sstorage_cmp_1.
+    
+    (* memory *)
+    unfold compare_smemory in E_smemory_cmp.
+    unfold safe_smemory_cmp in H_safe_smemory_cmp.
+    pose proof (H_safe_smemory_cmp ctx (get_memory_sst sst1) (get_memory_sst sst2) (get_maxidx_smap (get_smap_sst sst1)) (get_bindings_smap (get_smap_sst sst1)) (get_maxidx_smap (get_smap_sst sst2)) (get_bindings_smap (get_smap_sst sst2)) ops H_is_sat H_valid_sst1_sb H_valid_sst2_sb H_valid_smemory_sst1 H_valid_smemory_sst2 E_smemory_cmp) as H_safe_smemory_cmp.
+
+    pose proof (H_safe_smemory_cmp model mem strg exts H_is_model) as H_safe_smemory_cmp.
+    destruct H_safe_smemory_cmp as [mem' [H_safe_smemory_cmp_0 H_safe_smemory_cmp_1]].
+    rewrite H_safe_smemory_cmp_0.
+    rewrite H_safe_smemory_cmp_1.
+
+    (* stack *)
+    unfold compare_sstack in E_sstack_cmp.
+
+    pose proof (sstack_cmp_snd sstack_val_cmp ctx (get_stack_sst sst1) (get_stack_sst sst2) (get_maxidx_smap (get_smap_sst sst1)) (get_bindings_smap (get_smap_sst sst1)) (get_maxidx_smap (get_smap_sst sst2)) (get_bindings_smap (get_smap_sst sst2)) ops H_is_sat H_valid_sstack_sst1 H_valid_sstack_sst2 H_valid_sst1_sb H_valid_sst2_sb H_safe_sstack_val_cmp E_sstack_cmp) as H_sstack_cmp_snd.
+      
+    pose proof (H_sstack_cmp_snd model mem strg exts H_is_model) as H_sstack_cmp_snd.
+    destruct H_sstack_cmp_snd as [v [H_eval_sstk1 H_eval_sstk2]].
+    rewrite H_eval_sstk1.
+    rewrite H_eval_sstk2.
+    
+    exists (make_st v mem' strg' exts).
+    split; reflexivity.
+Qed.
+    
+
+End SymbolicStateCmpSoundness.
